minisepcomp/mini_diagram_trans_MatchInfo.v
@@ -25,6 +25,8 @@ Ltac exact_eq H :=
     |- ?p -> ?q => cut (p = q); [intros ->; auto | ]
   end.
 
+Lemma EQTRIV {A B: Type} (f g : A -> B) (H: f = g) a: f a = g a.
+Proof. subst; trivial. Qed.
 
 Lemma freshblock_forward m1 m2 m3 b: mem_forward m2 m3 -> freshblock m1 m2 b = true -> freshblock m1 m3 b = true.
 Proof. intros. apply freshblockProp_char. apply freshblockProp_char in H0.
@@ -47,8 +49,107 @@ Context {F1 V1 C1 F2 V2 C2 F3 V3 C3:Type}
         (g1 : Genv.t F1 V1)
         (g2 : Genv.t F2 V2)
         (g3 : Genv.t F3 V3).
-(*
+
 Lemma ext_inj_diagram: forall 
+(core_data12 : Type)
+(match_core12 : core_data12 -> C1 -> mem -> MatchInfoE -> C2 -> mem -> Prop)
+(core_ord12 : core_data12 -> core_data12 -> Prop)
+(senvs_dom_eq12 : Senv.equiv g1 g2 /\ genv_next_eq g1 g2)
+(match_wd12 : forall (d : core_data12) (c1 : C1) (m1 : mem) (M1 : block -> Z -> bool)
+               (L : block -> bool) (M2 : block -> Z -> bool) (c2 : C2) 
+               (m2 : mem),
+             match_core12 d c1 m1 (M1, L, M2) c2 m2 ->
+             forall b : block, L b = true -> Mem.valid_block m1 b /\ Mem.valid_block m2 b)
+(effcore_diagram12 : forall (st1 : C1) (m1 : mem) (st1' : C1) (m1' : mem)
+                      (U1 : block -> Z -> bool),
+                    effstep Sem1 g1 U1 st1 m1 st1' m1' ->
+                    forall (cd : core_data12) (st2 : C2) (m2 : mem) 
+                      (M1 : block -> Z -> bool) (L : block -> bool) 
+                      (M2 : block -> Z -> bool),
+                    match_core12 cd st1 m1 (M1, L, M2) st2 m2 ->
+                    exists
+                      (st2' : C2) (m2' : mem) (cd' : core_data12) (U2 : block -> Z -> bool),
+                      (effstep_plus Sem2 g2 U2 st2 m2 st2' m2' \/
+                       effstep_star Sem2 g2 U2 st2 m2 st2' m2' /\ core_ord12 cd' cd) /\
+                      (let L' := fun b : block => L b || freshblock m1 m1' b in
+                       let M1' :=
+                         fun (b : block) (z : Z) =>
+                         valid_block_dec m1 b && negb (L b) && (M1 b z || U1 b z) in
+                       let M2' :=
+                         fun (b : block) (z : Z) =>
+                         valid_block_dec m2 b && negb (L b) && (M2 b z || U2 b z) in
+                       L' = (fun b : block => L b || freshblock m2 m2' b) /\
+                       match_core12 cd' st1' m1' (M1', L', M2') st2' m2'))
+(core_data23 : Type)
+(match_core23 : core_data23 ->
+               meminj -> MatchInfo -> C2 -> mem -> MatchInfo -> C3 -> mem -> Prop)
+(core_ord23 : core_data23 -> core_data23 -> Prop)
+(match_wd23 : forall (d : core_data23) (j : meminj) (M1 : block -> Z -> bool)
+               (L1 : block -> bool) (c1 : C2) (m1 : mem) (M2 : block -> Z -> bool)
+               (L2 : block -> bool) (c2 : C3) (m2 : mem),
+             match_core23 d j (M1, L1) c1 m1 (M2, L2) c2 m2 ->
+             forall (b1 b2 : block) (d0 : Z), j b1 = Some (b2, d0) -> L1 b1 = L2 b2)
+(match_valid23 : forall (d : core_data23) (j : meminj) (E1 : MatchInfo) 
+                  (c1 : C2) (m1 : mem) (E2 : MatchInfo) (c2 : C3) (m2 : mem),
+                match_core23 d j E1 c1 m1 E2 c2 m2 -> meminj_valid j E1 E2 m1 m2)
+(effcore_diagram23 : forall (st1 : C2) (m1 : mem) (st1' : C2) (m1' : mem)
+                      (U1 : block -> Z -> bool),
+                    effstep Sem2 g2 U1 st1 m1 st1' m1' ->
+                    forall (cd : core_data23) (st2 : C3) (j : meminj) 
+                      (m2 : mem) (E1 E2 : MatchInfo),
+                    match_core23 cd j E1 st1 m1 E2 st2 m2 ->
+                    exists
+                      (st2' : C3) (m2' : mem) (cd' : core_data23) (j' : meminj) 
+                    (U2 : block -> Z -> bool),
+                      (effstep_plus Sem3 g3 U2 st2 m2 st2' m2' \/
+                       effstep_star Sem3 g3 U2 st2 m2 st2' m2' /\ core_ord23 cd' cd) /\
+                      (let (M1, L1) := E1 in
+                       let (M2, L2) := E2 in
+                       let L1' := fun b : block => L1 b || freshblock m1 m1' b in
+                       let L2' := fun b : block => L2 b || freshblock m2 m2' b in
+                       let M1' :=
+                         fun (b : block) (z : Z) =>
+                         valid_block_dec m1 b && negb (L1 b) && (M1 b z || U1 b z) in
+                       let M2' :=
+                         fun (b : block) (z : Z) =>
+                         valid_block_dec m2 b && negb (L2 b) && (M2 b z || U2 b z) in
+                       mini_intern_incr j j' L1' L2' /\
+                       globals_separate m1 g3 j j' /\
+                       match_core23 cd' j' (M1', L1') st1' m1' (M2', L2') st2' m2'))
+(st1 : C1) (m1 m2 m3 m1': mem) (st1' : C1)
+(U1 : block -> Z -> bool)
+(CS1 : effstep Sem1 g1 U1 st1 m1 st1' m1')
+(d12 : core_data12)
+(d23 : core_data23)
+(st3 : C3)
+(j : meminj)
+(M1 M2 M3 : block -> Z -> bool)
+(L1 L3 : block -> bool)
+(c2 : C2)
+(MC12 : match_core12 d12 st1 m1 (M1, L1, M2) c2 m2)
+(MC23 : match_core23 d23 j (M2, L1) c2 m2 (M3, L3) st3 m3),
+exists
+  (st2' : C3) (m2' : mem) (cd' : core_data12 * option C2 * core_data23) 
+(j' : meminj) (U2 : block -> Z -> bool),
+  (effstep_plus Sem3 g3 U2 st3 m3 st2' m2' \/
+   effstep_star Sem3 g3 U2 st3 m3 st2' m2' /\
+   clos_trans (core_data12 * option C2 * core_data23)
+     (sem_compose_ord_eq_eq core_ord12 core_ord23 C2) cd' (d12, Some c2, d23)) /\
+  (let L1' := fun b : block => L1 b || freshblock m1 m1' b in
+   let L2' := fun b : block => L3 b || freshblock m3 m2' b in
+   let M1' :=
+     fun (b : block) (z : Z) => valid_block_dec m1 b && negb (L1 b) && (M1 b z || U1 b z) in
+   let M2' :=
+     fun (b : block) (z : Z) => valid_block_dec m3 b && negb (L3 b) && (M3 b z || U2 b z) in
+   mini_intern_incr j j' L1' L2' /\
+   globals_separate m1 g3 j j' /\
+   (let (y, d2) := cd' in
+    let (d1, X) := y in
+    exists (c0 : C2) (m0 : mem) (M0 : block -> Z -> bool),
+      X = Some c0 /\
+      match_core12 d1 st1' m1' (M1', L1', M0) c0 m0 /\
+      match_core23 d2 j' (M0, L1') c0 m0 (M2', L2') st2' m2')).
+(*
 (GNE12: genv_next_eq g1 g2)
 (core_data12 : Type)
 (match_core12 : core_data12 -> C1 -> mem -> (block -> bool) -> C2 -> mem -> Prop)
@@ -133,22 +234,38 @@ exists
       U3 b2 ofs = true ->
       L3 b2 = true \/
       (exists (b1 : block) (delta : Z),
-         j b1 = Some (b2, delta) /\ U1 b1 (ofs - delta) = true))).
+         j b1 = Some (b2, delta) /\ U1 b1 (ofs - delta) = true))).*)
 Proof. intros.
-  destruct (effcore_diagram12 _ _ _ _ _ CS1 _ _ _ _ MC12)
-    as [st2' [m2' [d12' [L1' [HL1' [HL2' [MC12' [U2 [Y MOD12]]]]]]]]]; clear effcore_diagram12.
-  assert (ZZ: effstep_plus Sem2 g2 U2 st2 m2 st2' m2' \/
-    (st2,m2) = (st2',m2') /\ core_ord12 d12' d12).
-  destruct Y. auto.
-  destruct H.
-  destruct H. destruct x.
-  right. simpl in H. destruct H. split; auto.
-  left. exists x; auto.
-  clear Y. destruct ZZ as [CS2 | [CS2 ord12']].
+  exploit effcore_diagram12. apply CS1. apply MC12.
+  intros [st2' [m2' [d12' [U2 [STEPS2 [HL' MC12']]]]]]; clear effcore_diagram12.  
+  assert (ZZ: effstep_plus Sem2 g2 U2 c2 m2 st2' m2' \/
+    (c2,m2) = (st2',m2') /\ U2 = (fun b z => false) /\ core_ord12 d12' d12).
+  { destruct STEPS2. auto.
+    destruct H.
+    destruct H. destruct x.
+    right. simpl in H. destruct H. split; auto.
+    left. exists x; auto. }
+  clear STEPS2. destruct ZZ as [CS2 | [CS2 [HU2 ord12']]].
  (*case1*) 
 + destruct CS2.
   clear CS1. 
   cut (exists st3' : C3,  exists m3' : mem, 
+    exists d23':core_data23, exists j', exists U3,
+      (effstep_plus Sem3 g3 U3 st3 m3 st3' m3' \/
+        (effstep_star Sem3 g3 U3 st3 m3 st3' m3' /\
+        clos_trans (core_data12 * option C2 * core_data23)
+        (sem_compose_ord_eq_eq core_ord12 core_ord23 C2) 
+               (d12', Some st2', d23')
+        (d12, Some c2,d23)))
+    /\ let L2' := fun b : block => L1 b || freshblock m2 m2' b in
+       let L3' := fun b : block => L3 b || freshblock m3 m3' b in
+       let M2' := (fun b z => valid_block_dec m2 b && negb (L1 b) && (M2 b z || U2 b z)) in
+       let M3' := (fun b z => valid_block_dec m3 b && negb (L3 b) && (M3 b z || U3 b z)) in
+      mini_intern_incr j j' L2' L3' 
+    /\  globals_separate m2 g3 j j'
+    (*/\mini_locally_allocated L1 L3 m2 m3 L22' L3' m2' m3'*)
+    /\ match_core23 d23' j' (M2',L2') st2' m2' (M3',L3') st3' m3').    
+(*  cut (exists st3' : C3,  exists m3' : mem, 
     exists d23':core_data23, exists j', exists L22', exists L3',
       mini_intern_incr j j' L22' L3' /\
       globals_separate m2 g3 j j' /\
@@ -166,72 +283,55 @@ Proof. intros.
       U3 b3 ofs = true ->
       L3 b3 = true \/
       (exists (b2 : block) (delta : Z),
-         j b2 = Some (b3, delta) /\ U2 b2 (ofs - delta) = true)))).
-  - intros [st3' [m3' [d23' [j' [L22' [L3' (*[INV'*) [InjIncr23 
-          [Gsep23 [LocAlloc23 [MC23' [U3 [ZZ MOD23]]]]]]]]]]]].
+         j b2 = Some (b3, delta) /\ U2 b2 (ofs - delta) = true)))).*)
+
+  - intros [st3' [m3' [d23' [j' [U3 [STEP3 (*[INV'*) [InjIncr23
+          [Gsep23 MC23']]]]]]]]. 
     exists st3'. exists m3'. 
     exists (d12', Some st2', d23').
-    exists j', L1', L3'.
-    assert (L22' = L1').
-    { clear - HL2' LocAlloc23. destruct LocAlloc23. subst. reflexivity. }
-    subst L22'.
+    exists j', U3.
     split. assumption.
-    split. { clear ZZ MOD23. red; intros. destruct (Gsep23 _ _ _ J J'); clear Gsep23. split; trivial.
+    split. { destruct InjIncr23 as [INC23a INC23b].
+      split; trivial.
+      intros b2 b3 d; intros.
+        destruct (INC23b _ _ _ J J'). split; trivial.
+        rewrite (EQTRIV _ _ HL'); trivial. }
+    split. { red; intros. destruct (Gsep23 _ _ _ J J'); clear Gsep23. split; trivial.
              intros N. elim H0; clear H0. destruct InjIncr23 as [INC SEP].
              destruct (SEP _ _ _ J J').
-             assert ((fun b : block => L1 b || freshblock m1 m1' b) b1 = true). rewrite HL1' in H0; trivial. clear HL1'; simpl in H3; subst L1'.
-             case_eq (L1 b1); intros ZZ; rewrite ZZ in *; simpl in  *. apply (match_localblocks12 _ _ _ _ _ _ MC12 _ ZZ).
+             assert ((fun b : block => L1 b || freshblock m1 m1' b) b1 = true). rewrite (EQTRIV _ _ HL'); trivial.
+             simpl in H3.
+             case_eq (L1 b1); intros ZZ; rewrite ZZ in *; simpl in  *. eapply match_wd12; eauto.
              apply freshblockProp_char in H3. destruct H3; congruence. }
-    split. { split. assumption. destruct LocAlloc23. assumption. }  
-    split.
-    { exists st2', m2'. clear ZZ. intuition. }  
-    exists U3. split. apply ZZ. 
-    intros. 
-    assert (M12H: forall (b2 : block) (z : Z), U2 b2 z = true -> L1 b2 = true \/ j b2 <> None).
-    { intros. destruct (MOD12 _ _ H2); [ left; trivial |  apply (H0 _ _ H3)]. }
-    destruct (MOD23 M12H _ _ H1); clear M12H MOD23.
-    * left; trivial.
-    * destruct H2 as [b1 [d [? ?]]].
-      destruct (MOD12 _ _ H3).
-      solve [ left; rewrite <- (match_wd23 _ _ _ _ _ _ _ _ MC23 _ _ _ H2); trivial].
-      right; exists b1, d; split; trivial.
+    exists st2', m2'; eexists. split. trivial. rewrite <- HL' in MC23'. split; eassumption.
   -  
-  clear MC12 MC12' HL1' MOD12. 
-  clear st1 m1 st1' m1' GNE12. 
-  clear match_localblocks12 C1 Sem1 match_core12 g1 U1. clear HL2' HL2' L1'.
-  revert U2 j d23 st2 m2 st3 m3 H L1 L3 MC23. 
+  clear MC12 MC12' HL'.
+  clear st1 m1 st1' m1'. 
+  clear senvs_dom_eq12 match_wd12 C1 Sem1 match_core12 g1 U1 M1. 
+  revert U2 j d23 c2 m2 st3 m3 H M2 L1 M3 L3 MC23. 
   induction x; intros. 
   {
    (*base case*) simpl in H.
-    destruct H as [c2 [m2'' [U3 [U4 [? [? ?]]]]]].
-    destruct H0. inv H0; simpl in *. 
-    destruct (effcore_diagram23 _ _ _ _ _ H _ _ _ _ _ _ MC23) 
-      as [st3' [m3' [d23' [j23' [L22' [L3' [InjIncr23 
-          [Gsep23 [LocAlloc23 [MC23' [U5 [? MOD32]]]]]]]]]]]]; clear effcore_diagram23.
-    exists st3'. exists m3'. exists d23'. exists j23', L22', L3'. 
+    destruct H as [st2 [m2'' [U3 [U4 [? [[? ?] ?]]]]]]. subst U4. simpl in H2.
+    assert (U2 = U3). { subst U2. extensionality b. extensionality z. apply orb_false_r. }
+    clear H2. subst U2. inv H0. simpl in *. 
+    exploit effcore_diagram23. apply H. apply MC23.
+    intros [st3' [m3' [d23' [j23' [U5 [STEPS3 [InjIncr23 
+          [Gsep23 MC23' ]]]]]]]]; clear effcore_diagram23.
+    exists st3'. exists m3'. exists d23', j23', U5. 
+    split. { destruct STEPS3. left; assumption.
+             destruct H0. right. split; trivial.
+             apply t_step. constructor 2. apply H1. }
     split. trivial. 
-    split. trivial. 
-    split. trivial. 
-    split. trivial. 
-    exists U5. 
-    split. destruct H0. left; assumption.
-           destruct H0. right. split; trivial.
-           apply t_step. constructor 2. apply H1.
-    intros.  
-      assert (U3Hyp': forall b1 z, U3 b1 z = true -> L1 b1 = true \/ j b1 <> None).
-      { intros. eapply (H1 b1 z). rewrite H3; trivial. }
-      clear H1.
-      destruct (MOD32 U3Hyp' _ _ H2). left; trivial. 
-      destruct H1 as [? [? [? ?]]].
-      right. exists x, x0. rewrite H3. split; trivial. }
+    split; trivial. }
   {
    (*inductive case*)
     remember (S x) as x'. simpl in H.
     rename st2' into st2''. rename m2' into m2''.
     destruct H as [st2' [m2' [U4 [U3 [Step2 [StepN2 HU]]]]]]. subst x'.
-    destruct (effcore_diagram23 _ _ _ _ _ Step2 _ _ _ _ _ _ MC23) 
-      as [c3' [m3' [d23' [j23' [L2a' [L3a' [InjInc23  
-             [Gsep23 [LocAlloc23 [MC23' [U5 [Steps3 MOD23]]]]]]]]]]]]; clear effcore_diagram23.
+    exploit effcore_diagram23. apply Step2. apply MC23.
+    intros [c3' [m3' [d23' [j23' [U5 [Steps3 [InjInc23  
+             [Gsep23  MC23']]]]]]]]; clear effcore_diagram23.
     assert (FWD2: mem_forward m2 m2').
         eapply effstep_fwd; eassumption.
     assert (FWD2': mem_forward m2' m2'').
@@ -239,40 +339,15 @@ Proof. intros.
     assert (FWD3: mem_forward m3 m3').
         destruct Steps3 as [[n K] | [[n K] _]];
              eapply effstepN_fwd; eassumption.
-    destruct (IHx _ j23' d23' _ _ c3' m3' StepN2 _ _ MC23') 
-        as [c3'' [m3'' [d23'' [j23'' [LL2 [LL3 [InjIncr' 
-             [Gsep' [LocAlloc23' [MC23'' [U3' [StepN3 MOD23']]]]]]]]]]]]; clear IHx.
+    exploit (IHx _ j23' d23' _ _ c3' m3' StepN2). apply MC23'. 
+    intros [c3'' [m3'' [d23'' [j23'' [U3' [StepN3 [InjIncr' 
+             [Gsep' MC23'']]]]]]]]; clear IHx.
     assert (FWD3': mem_forward m3' m3'').
         destruct StepN3 as [[n K] | [[n K] _]];
              eapply effstepN_fwd; eassumption.
-    exists c3''. exists m3''. exists d23''. exists j23'', LL2, LL3.
-    split. { (*mini_intern_trans*) clear - InjIncr' InjInc23 LocAlloc23'.
-             destruct InjIncr'; destruct InjInc23. destruct LocAlloc23'; subst.
-             split. eapply inject_incr_trans; eassumption.
-             intros. remember(j23' b1) as q.
-             destruct q; symmetry in Heqq.
-             + destruct p. specialize (H _ _ _ Heqq). rewrite J' in H. inv H.
-               destruct (H2 _ _ _ J Heqq). rewrite H, H3; simpl. split; trivial.
-             + apply (H0 _ _ _ Heqq J'). } 
-    split. { clear - InjIncr' InjInc23 Gsep' Gsep23 FWD2.
-             destruct InjIncr'; destruct InjInc23. 
-             red; intros. remember(j23' b1) as q.
-             destruct q; symmetry in Heqq.
-             + destruct p. specialize (H _ _ _ Heqq). rewrite J' in H. inv H.
-               apply (Gsep23 _ _ _ J Heqq). 
-             + destruct (Gsep' _ _ _ Heqq J'). split; trivial.
-               intros N. elim H3; clear H3. apply FWD2; eauto. }
-    split. { specialize (freshblock_trans _ _ _ FWD2 FWD2'); intros FW2.
-             specialize (freshblock_trans _ _ _ FWD3 FWD3'); intros FW3.
-             clear - FW2 FW3 LocAlloc23 LocAlloc23'.
-             destruct LocAlloc23; subst. destruct LocAlloc23'; subst.
-             split; extensionality b. 
-             + rewrite <- orb_assoc, FW2; trivial.
-             + rewrite <- orb_assoc, FW3; trivial. }
-    split. apply MC23''.
-    exists (fun b z => U5 b z || (U3' b z && valid_block_dec m3 b)). 
-    split. clear MOD23 MOD23'. 
-           destruct Steps3; destruct StepN3.
+    exists c3'', m3'', d23'', j23''. 
+    exists (fun b z => U5 b z || (U3' b z && valid_block_dec m3 b)).
+    split. { destruct Steps3; destruct StepN3.
            (*1/4*)
               left. eapply effstep_plus_trans; eassumption.
            (*2/4*)
@@ -288,72 +363,100 @@ Proof. intros.
                eapply t_trans.
                  apply CT. clear CT.  
                  apply t_step.
-                 constructor 2. apply CORD.
-    (*MOD23-clause*) subst U2. intros U4Hyp b3 ofs HU3.
-      apply orb_true_iff in HU3.
-      destruct HU3.
-      - assert (U4Hyp': forall b1 z, U4 b1 z = true -> L1 b1 = true \/ j b1 <> None).
-        { intros. apply (U4Hyp b1 z). rewrite H0; trivial. }
-        destruct (MOD23 U4Hyp' _ _ H). left; trivial.
-        right. destruct H0 as [? [? [? ?]]]. exists x0, x1; rewrite H1; split; trivial.
-      - apply andb_true_iff in H. destruct H.
-         destruct (valid_block_dec m3 b3); try inv H0.
-         assert (U3Hyp: forall b z, U3 b z = true -> L2a' b = true \/ j23' b <> None).
-         { intros. 
-           assert (U3valid:= effstepN_valid _ _ _ _ _ _ _ _ StepN2 _ _ H0).
-           specialize (U4Hyp b z). rewrite H0 in U4Hyp; simpl in U4Hyp.
-           destruct (valid_block_dec m2 b); simpl in U4Hyp.
-           * rewrite orb_true_r in U4Hyp.
-             destruct LocAlloc23; subst. 
-             destruct U4Hyp; trivial.
-             left. rewrite H1; trivial.
-             right. remember (j b) as q. destruct q; try solve [congruence].
-                    symmetry in Heqq; destruct p. destruct InjInc23 as [II _].
-                    rewrite (II _ _ _ Heqq). discriminate.
-           * rewrite orb_false_r in U4Hyp.
-             destruct LocAlloc23. subst. left.
-             assert (freshblockProp m2 m2' b) by (split; trivial).
-             rewrite freshblock_asProp in H1. unfold asProp in H1; rewrite H1; apply orb_true_r. 
-         }
-         destruct (MOD23' U3Hyp _ _ H); clear MOD23'.
-         * destruct LocAlloc23; subst.
-           apply orb_true_iff in H0. destruct H0. left; trivial.
-           apply freshblockProp_char in H0.
-           destruct H0. contradiction.
-         * destruct H0 as [? [? [? ?]]].
-           destruct InjInc23 as [II23a II23b].
-           remember (j x0) as q.
-           destruct q; symmetry in Heqq.
-           + destruct p; specialize (II23a _ _ _ Heqq). rewrite II23a in H0. inv H0.
-             right. exists x0, x1. split; trivial. rewrite H1. simpl.
-             destruct (match_valid23 _ _ _ _ _ _ _ _ MC23) as [A [ B C]].
-             destruct (C _ _ _ Heqq). destruct (valid_block_dec m2 x0); try contradiction. apply orb_true_r.
-           + destruct (II23b _ _ _ Heqq H0). destruct LocAlloc23; subst.
-             apply orb_true_iff in H3. destruct H3. left; trivial.
-             apply freshblockProp_char in H3.
-             destruct H3; contradiction.
+                 constructor 2. apply CORD. }
+   split. { (*mini_intern_trans*) clear - InjIncr' InjInc23 FWD3' FWD3 FWD2' FWD2.
+             destruct InjIncr'; destruct InjInc23. 
+             split. eapply inject_incr_trans; eassumption.
+             intros. case_eq (j23' b1); intros.
+             + destruct p. specialize (H _ _ _ H3). rewrite J' in H. inv H.
+               destruct (H2 _ _ _ J H3).
+               split.
+               - case_eq (L1 b1); intros Lb; rewrite Lb in *; simpl in *; trivial.
+                 eapply freshblock_forward; eassumption. 
+               - case_eq (L3 b); intros Lb; rewrite Lb in *; simpl in *; trivial.
+                 eapply freshblock_forward; eassumption.
+             + destruct (H0 _ _ _ H3 J').
+               split.
+               - case_eq (L1 b1); intros Lb; rewrite Lb in *; simpl in *; trivial.
+                 erewrite <- freshblock_trans; eassumption. 
+               - case_eq (L3 b2); intros Lb; rewrite Lb in *; simpl in *; trivial.
+                 erewrite <- freshblock_trans; eassumption. } 
+    split. { clear - InjIncr' InjInc23 Gsep' Gsep23 FWD2.
+             destruct InjIncr'; destruct InjInc23. 
+             red; intros. remember(j23' b1) as q.
+             destruct q; symmetry in Heqq.
+             + destruct p. specialize (H _ _ _ Heqq). rewrite J' in H. inv H.
+               apply (Gsep23 _ _ _ J Heqq). 
+             + destruct (Gsep' _ _ _ Heqq J'). split; trivial.
+               intros N. elim H3; clear H3. apply FWD2; eauto. }
+    exact_eq MC23''; subst U2. f_equal.
+    + f_equal.
+      - extensionality bb. extensionality z.
+        case_eq (L1 bb); simpl; intros.
+        * repeat rewrite andb_false_r; simpl; trivial.
+        * rewrite andb_true_r.
+          case_eq (valid_block_dec m2 bb); simpl; intros.
+          ++ rewrite andb_true_r, orb_assoc.
+             case_eq (valid_block_dec m2' bb); simpl; intros.
+             2: elim n; apply FWD2; trivial.
+             assert (FR2: freshblock m2 m2' bb = false). apply freshblock_charF; left; trivial.
+             rewrite FR2; simpl. trivial.
+          ++ case_eq (U3 bb z); simpl; intros. 2: rewrite andb_false_r; trivial.
+             assert (Mem.valid_block m2' bb). 
+             { eapply effstepN_valid. apply StepN2. apply H1. }
+             case_eq (valid_block_dec m2' bb); simpl; intros; try contradiction.
+             assert (FR2: freshblock m2 m2' bb = true). eapply freshblockProp_char. split; trivial.
+             rewrite FR2; simpl; trivial.
+      - extensionality bb. rewrite <- (freshblock_trans m2 m2' m2''), orb_assoc; trivial.
+    + f_equal.
+      - extensionality bb. extensionality z.
+        case_eq (L3 bb); simpl; intros.
+        * repeat rewrite andb_false_r; simpl; trivial.
+        * rewrite andb_true_r.
+          case_eq (valid_block_dec m3 bb); simpl; intros.
+          ++ rewrite andb_true_r, orb_assoc.
+             case_eq (valid_block_dec m3' bb); simpl; intros.
+             2: elim n; apply FWD3; trivial.
+             assert (FR3: freshblock m3 m3' bb = false). apply freshblock_charF; left; trivial.
+             rewrite FR3; simpl. trivial.
+          ++ case_eq (U3' bb z); simpl; intros. 2: rewrite andb_false_r; trivial.
+             assert (Mem.valid_block m3' bb). 
+             { destruct StepN3 as [[nn StepNN] | [[nn StepNN] _]]; eapply effstepN_valid.
+               apply StepNN. eassumption. apply StepNN. eassumption. }
+             case_eq (valid_block_dec m3' bb); simpl; intros; try contradiction.
+             assert (FR3: freshblock m3 m3' bb = true). eapply freshblockProp_char. split; trivial.
+             rewrite FR3; simpl; trivial.
+      - extensionality bb. rewrite <- (freshblock_trans m3 m3' m3''), orb_assoc; trivial.
   }
 +
   (*case 2*)
-   inversion CS2; clear CS2. subst st2 m2.
-   assert (L1' = L1).
-   { rewrite HL2'. extensionality b. rewrite freshblock_irrefl; apply orb_false_r. } 
-   clear HL2'. rewrite H in *. clear H L1'.  
-   exists st3. exists m3.
-   exists (d12',Some st2',d23), j, L1, L3.
+   inversion CS2; clear CS2. subst st2' m2' U2.  
+   exists st3, m3, (d12',Some c2,d23), j, (fun b z => false). 
+   split. { right. split. exists O. simpl; auto.
+            apply t_step. constructor 1; auto. }
    split. { split; intros. apply inject_incr_refl. congruence. }
    split. { red; intros; congruence. }
-   split. { split; trivial.
-            extensionality b. rewrite freshblock_irrefl, orb_false_r; trivial. }
-   split.
-   { clear effcore_diagram23.
-     exists st2'. exists m2'. repeat split; auto. }
-
-   exists (fun b z => false). 
-    split. right. split. exists O. simpl; auto.
-    apply t_step. constructor 1; auto. intros; discriminate.
+   exists c2, m2. eexists. split. trivial.
+   split. eassumption.
+   exploit match_valid23. apply MC23. intros MV.
+   exact_eq MC23. f_equal.
+       - f_equal.
+         * extensionality b. extensionality z. rewrite orb_false_r.
+           destruct MV as [MVa [MVb [MVc [MVd MVe]]]].
+           case_eq (M2 b z); simpl; intros.
+           -- destruct (MVd _ _ H) as [X Y]; rewrite Y; simpl.
+             destruct (valid_block_dec m2 b); trivial. contradiction.
+           -- rewrite andb_false_r; trivial.
+         * rewrite HL'. extensionality b. rewrite freshblock_irrefl', orb_false_r; trivial. 
+       - f_equal; extensionality b.
+         -- extensionality z. rewrite orb_false_r.
+            destruct MV as [MVa [MVb [MVc [MVd MVe]]]].
+            case_eq (M3 b z); simpl; intros.
+            ++ destruct (MVe _ _ H) as [X Y]; rewrite Y; simpl.
+               destruct (valid_block_dec m3 b); trivial. contradiction.
+            ++ rewrite andb_false_r; trivial.
+         -- rewrite freshblock_irrefl, orb_false_r; trivial.
 Qed.
-*)
 
 Lemma effcore_diagram_trans: forall
 (core_data12 : Type)
