minisepcomp/transEI_MatchInfo.v
@@ -16,19 +16,29 @@ Require Import sepcomp.effect_semantics.
 
 Require Import msl.Axioms. (*for extensionality*)
 
-Require Import minisepcomp.mini_simulations.
-Require Import minisepcomp.mini_simulations_lemmas.
+Require Import minisepcomp.mini_simulations_MatchInfo.
+Require Import minisepcomp.mini_simulations_lemmas_MatchInfo.
 Require Import Wellfounded.
 Require Import Relations.
-Require Import minisepcomp.mini_diagram_trans. (*for compose_ord_eq_eq*)
-(*Require Import minisepcomp.interpolation_memory.*)
-Require Import minisepcomp.mem_interpolation_EI.
+Require Import minisepcomp.mini_diagram_trans_MatchInfo. (*for compose_ord_eq_eq*)
+Require Import minisepcomp.mem_interpolation_EI_MatchInfo.
 
 Require Import minisepcomp.BuiltinEffects.
 
 Import Mini_simulation_inj.
 
 Import Mini_simulation_ext.
+
+Lemma EffectsPropagate_EI j M1 M3 M2
+      (EProp2 : EffectsPropagateE M1 M2)
+      (EProp3 : EffectsPropagate j M2 M3):
+  EffectsPropagate j M1 M3.
+Proof. red; intros.  red in EProp2. red in EProp3.
+    assert (X: forall b2 z, M2 b2 z = true -> j b2 <> None) by eauto.
+    destruct (EProp3 X _ _ Ub) as [b1 [d [J Hb1]]].
+    exists b1, d; split; trivial. eauto.
+Qed.
+
 (*
 Lemma initial_inject_split: forall j m1 m3 (Inj:Mem.inject j m1 m3),
   exists m2 j1 j2, j = compose_meminj j1 j2 /\
@@ -75,21 +85,22 @@ Proof.
       core_halted23 core_at_external23 eff_after_external23].
   eapply Build_Mini_simulation_inject with
     (core_ord := clos_trans _ (sem_compose_ord_eq_eq core_ord12 core_ord23 C2))
-    (match_state := fun d j L1 c1 m1 L3 c3 m3 => 
+    (match_state := fun d j E1 c1 m1 E3 c3 m3 => 
       match d with (d1,X,d2) => 
-        exists c2, exists m2, 
+        exists c2, exists m2, exists M2,
           X=Some c2 /\ 
-          match_core12 d1 c1 m1 L1 c2 m2 /\ match_core23 d2 j L1 c2 m2 L3 c3 m3 (*/\
-          full_ext j1 j2 L1 L2*)
+          match E1 with (M1, L1) =>
+          match_core12 d1 c1 m1 (M1,L1,M2) c2 m2 /\ match_core23 d2 j (M2,L1) c2 m2 E3 c3 m3
+          end
       end).
 { (*well_founded*)
   eapply wf_clos_trans. 
   eapply well_founded_sem_compose_ord_eq_eq; assumption. }
 { (*match_wd*) clear - match_wd12 match_wd23.
   intros. rename c2 into c3. rename m2 into m3. rename L2 into L3. rename b2 into b3.
-  destruct d as [[d12 cc2] d23].
-  destruct MS as [c2 [m2 [X [MC12 MC23]]]]; subst.
-  eapply (match_wd23 _ _ _ _ _ _ _ _ MC23); eassumption. }
+  destruct d as [[d12 cc2] d23]. rename M2 into M3.
+  destruct MS as [c2 [m2 [M2 [X [MC12 MC23]]]]]; subst.
+  eapply (match_wd23 _ _ _ _ _ _ _ _ _ _ MC23); eassumption. }
 { (*senvs_domain_eq*)
   clear - senvs_dom_eq12 senvs_dom_eq23. destruct senvs_dom_eq12. 
    eapply senv_equiv_trans; eauto. }
@@ -106,10 +117,11 @@ Proof.
     destruct (Genv.find_var_info g2 b); try contradiction.
   apply GfindSymb23. apply GfindSymb12. assumption. }*)
 { (*match_genv*)
-  intros. rename c2 into c3. rename m2 into m3. rename L2 into L3.
-  destruct d as [[d12 cc2] d23].
-  destruct MC as [c2 [m2  [X [MC12 MC23 ]]]]; subst.
-  destruct (match_genv12 _ _ _ _ _ _ MC12) as [GE12a [GE12b GE12c]].
+  clear - match_genv23 match_genv12 match_valid23 match_valid12.
+  intros. rename c2 into c3. rename m2 into m3. destruct E2 as [M3 L3]. 
+  destruct d as [[d12 cc2] d23]. destruct E1 as [M1 L1].
+  destruct MC as [c2 [m2 [M2 [X [MC12 MC23 ]]]]]; subst.
+  destruct (match_genv12 _ _ _ _ _ _ _ _ MC12) as [GE12a [GE12b GE12c]].
   destruct (match_genv23 _ _ _ _ _ _ _ _ MC23) as [GE23a [GE23b GE23c]].
   assert (EQ: compose_meminj (Mem.flat_inj (Mem.nextblock m1)) j = j).
     { extensionality b. unfold compose_meminj.
@@ -119,7 +131,8 @@ Proof.
         destruct Heqq as [? [? ?]]; subst. simpl.
         remember (j b) as w; destruct w; trivial. destruct p; trivial.
       + remember (j b) as w. destruct w; trivial. symmetry in Heqw; destruct p.
-        eapply match_valid23 in Heqw; try eassumption. destruct Heqw.
+        destruct (match_valid23 _ _ _ _ _ _ _ _ MC23) as [MV23a [MV23b [MV23c [MV23d MV23e]]]].
+        destruct (MV23c _ _ _ Heqw).
         eapply match_valid12 in H; try eassumption.
         erewrite flatinj_I in Heqq; try discriminate. apply H. }
   split; [| split].
@@ -135,20 +148,27 @@ Proof.
 
 { (*meminj_valid*)
     clear - match_valid12 match_valid23.
-    intros. rename c2 into c3. rename m2 into m3. rename L2 into L3. 
-    destruct d as [[d12 cc2] d23].
-    destruct MS as [c2 [m2 [X [MC12 MC23]]]]; subst.
-    specialize (match_valid12 _ _ _ _ _ _ MC12).
-    specialize (match_valid23 _ _ _ _ _ _ _ _ MC23).
-    destruct match_valid23 as [MC23a [MC23b MC23c]].
-    split; intros. apply match_valid12; eauto.
-    split; intros. eauto.
-    destruct (MC23c _ _ _ J); split; eauto. apply match_valid12; trivial. }
+    intros. rename c2 into c3. rename m2 into m3. destruct E2 as [M3 L3]. 
+    destruct d as [[d12 cc2] d23]. destruct E1 as [M1 L1].
+    destruct MS as [c2 [m2 [M2 [X [MC12 MC23]]]]]; subst.
+    specialize (match_valid12 _ _ _ _ _ _ _ _ MC12).
+    specialize (match_valid23 _ _ _ _ _ _ _ _ MC23). red in match_valid23.
+    destruct match_valid23 as [MV23a [MV23b [MV23c [MV23d MV23e]]]].
+    destruct match_valid12 as [MV12a [MV12b MV12c]]. 
+    repeat split; intros.
+    - apply MV12a. apply MV23a; trivial.
+    - apply MV23b; trivial.
+    - apply MV12a. eapply MV23c; eassumption.
+    - eapply MV23c; eassumption.
+    - eapply MV12b; eauto.
+    - eapply MV12b; eauto.
+    - eapply MV23e; eauto.
+    - eapply MV23e; eauto. }
 { (*initial_core *)
   clear eff_after_external23 eff_after_external12 core_at_external23 core_at_external12.
   clear core_halted23 core_halted12 effcore_diagram23 effcore_diagram12. 
   intros. rename m2 into m3. rename vals2 into vals3. 
-  assert (MR2: mem_respects_readonly g2 m1). { admit. (*TODO: add readonly-preservation caluse to sim_extends_def?*) }
+  assert (MR2: mem_respects_readonly g2 m1). { admit. (*TODO: add readonly-preservation clause to sim_extends_def?*) }
    destruct (core_initial12 _ _ _ _ _ _ H (forall_lessdef_refl vals1) (Mem.extends_refl m1)) as [cd12 [c2 [Ini2 MC12]]]; trivial.
    { destruct H2 as [PGa [PGb PGc]].
      repeat split; intros.
@@ -192,35 +212,38 @@ Proof.
      split. intros. rewrite B1, A11; trivial.
      split. intros. destruct H2. rewrite A11 in *. destruct (B2 _ _ _ _ H3 H4); subst. rewrite B1, A11; trivial.*) } 
    exists (cd12, Some c2, cd23), c3. split. assumption.
-   exists c2, m1. split; trivial. split; trivial. }
+   unfold EmptyInfo, EmptyInfoE in *. 
+   exists c2, m1, (fun b z => false). split; trivial. split; trivial. }
 { (*core diagram*) clear - match_wd12 senvs_dom_eq12 effcore_diagram23 match_valid23 match_wd23 effcore_diagram12.
-   intros. rename st2 into st3. rename m2 into m3. rename L2 into L3.
-   destruct cd as [[d12 cc2] d23].
-   destruct H0 as [c2 [m2 [X [MC12 MC23]]]]; subst.
+   intros. rename st2 into st3. rename m2 into m3. destruct E2 as [M3 L3].
+   destruct cd as [[d12 cc2] d23]. destruct E1 as [M1 L1].
+   destruct H0 as [c2 [m2 [M2 [X [MC12 MC23]]]]]; subst.
    eapply (ext_inj_diagram Sem1 Sem2 Sem3 g1 g2 g3); eassumption. }
 { (*halted*) 
   clear - core_halted12 core_halted23; intros. 
-  rename c2 into c3. rename m2 into m3.
-  destruct cd as [[cd12 X] cd23]. destruct H as [c2 [m2 [? [MC12 MC23]]]]; subst.
-  destruct (core_halted12 _ _ _ _ _ _ _ MC12 H0) as [v2 [LDef [DRO1 [RDO2 [Halted2 EXT12]]]]].
-  destruct (core_halted23 _ _ _ _ _ _ _ _ _ MC23 Halted2) as [v3 [INJ23 [RDO2' [RDO3 [Vinj Halted3]]]]].
+  rename c2 into c3. rename m2 into m3. rename M2 into M3. rename L2 into L3.
+  destruct cd as [[cd12 X] cd23]. destruct H as [c2 [m2 [M2 [? [MC12 MC23]]]]]; subst.
+  destruct (core_halted12 _ _ _ _ _ _ _ _ _ MC12 H0) as [v2 [LDef [DRO1 [RDO2 [Halted2 [EXT12 EProp2]]]]]].
+  destruct (core_halted23 _ _ _ _ _ _ _ _ _ _ _ MC23 Halted2) as [v3 [INJ23 [RDO2' [RDO3 [Vinj [Halted3 EProp3]]]]]].
   exists v3; split.
     eapply Mem.extends_inject_compose; eassumption.
   split. trivial. 
   split. trivial.
+  split. eapply val_lessdef_inject_compose; eassumption.
   split; trivial.
-  eapply val_lessdef_inject_compose; eassumption.  
+  eapply EffectsPropagate_EI; eassumption.
   }
 { (*at_external*)
   clear - core_at_external23 core_at_external12; intros.
-  rename c2 into st3. rename m2 into m3.
-  destruct cd as [[cd12 X] cd23]. destruct H as [st2 [m2 [? [MC12 MC23]]]]; subst.
+  rename c2 into st3. rename m2 into m3. rename M2 into M3. rename L2 into L3. 
+  destruct cd as [[cd12 X] cd23]. destruct H as [st2 [m2 [M2 [? [MC12 MC23]]]]]; subst.
   
-  destruct (core_at_external12 _ _ _ _ _ _ _ _ _ MC12 H0) as [EXT12 [RDO1 [RDO2 [args2 [Vals12 AtExt2]]]]].
-  destruct (core_at_external23 _ _ _ _ _ _ _ _ _ _ _ MC23 AtExt2) as [INJ23 [RDO2' [RDO3 [args3 [Vals23 AtExt3]]]]].
+  destruct (core_at_external12 _ _ _ _ _ _ _ _ _ _ _ MC12 H0) as [EXT12 [RDO1 [RDO2 [EProp2 [args2 [Vals12 AtExt2]]]]]].
+  destruct (core_at_external23 _ _ _ _ _ _ _ _ _ _ _ _ _ MC23 AtExt2) as [INJ23 [RDO2' [RDO3 [EProp3 [args3 [Vals23 AtExt3]]]]]].
   split. eapply Mem.extends_inject_compose; eassumption.
   split. trivial.
   split. trivial.
+  split. eapply EffectsPropagate_EI; eassumption.
   exists args3; split; trivial. eapply forall_val_lessdef_inject_compose; eassumption. }
 { (*after_external*) 
   clear - match_wd12 match_valid12 core_at_external12 
@@ -231,22 +254,24 @@ Proof.
   intros. rename st2 into st3. rename m2 into m3. rename L2 into L3. 
           rename vals2 into vals3'. rename m2' into m3'.
           rename RDO2 into RDO3. rename ret2 into ret3. rename HasTy2 into HasTy3.
+          rename M2 into M3.
   destruct cd as [[d12 cc2] d23].
-  destruct MatchMu as [st2 [m2 [X [MC12 MC23]]]].
-  assert (WDmu12:= match_wd12 _ _ _ _ _ _ MC12).
-  assert (WDmu23:= match_wd23 _ _ _ _ _ _ _ _ MC23).  
-  destruct (core_at_external12 _ _ _ _ _ _ _ _ _ MC12 AtExtSrc) as [EXT12 [RespRd1 [RespRd2 [vals2 [Vals12 AtExt2]]]]].
-  destruct (core_at_external23 _ _ _ _ _ _ _ _ _ _ _ MC23 AtExt2) as [INJ23 [RespRd2' [RespRd3 [vals3 [Vals23 AtExt3]]]]].
+  destruct MatchMu as [st2 [m2 [M2 [X [MC12 MC23]]]]].
+  assert (WDmu12:= match_wd12 _ _ _ _ _ _ _ _ MC12).
+  assert (WDmu23:= match_wd23 _ _ _ _ _ _ _ _ _ _ MC23).  
+  destruct (core_at_external12 _ _ _ _ _ _ _ _ _ _ _ MC12 AtExtSrc) as [EXT12 [RespRd1 [RespRd2 [EProp2 [vals2 [Vals12 AtExt2]]]]]].
+  destruct (core_at_external23 _ _ _ _ _ _ _ _ _ _ _ _ _ MC23 AtExt2) as [INJ23 [RespRd2' [RespRd3 [EProp3 [vals3 [Vals23 AtExt3]]]]]].
   rewrite AtExtTgt in AtExt3; inv AtExt3.
   clear core_at_external12 core_at_external23.
-  specialize (eff_after_external12 _ _ _ _ _ _ _ _ _ _ 
+  specialize (eff_after_external12 _ _ _ _ _ _ _ _ _ _ _ _
         MC12 AtExtSrc AtExt2 Vals12). 
-  specialize (eff_after_external23 _ _ _ _ _ _ _ _ _ _ _ _ _ _ INJ23
+  specialize (eff_after_external23 _ _ _ _ _ _ _ _ _ _ _ _ _ _ _ _ INJ23
         MC23 AtExt2 AtExtTgt Vals23).
+  destruct (match_valid12 _ _ _ _ _ _ _ _ MC12) as [MV12a [MV12b MV12c]].
   assert (GSep23: globals_separate m2 g3 j j').
   { red; intros. clear eff_after_external23 eff_after_external12.
     destruct (GSep _ _ _ J J'). split; trivial. intros N; apply H; clear H.
-    eapply match_valid12; eauto. }
+    eapply MV12a; eauto. }
   assert (INTER: exists m2', (*mini_extern_incr j12 j12' L1 L2 /\ mini_extern_incr j23 j23' L2 L3 /\
                              meminj_valid j12' L1 m1' L2 m2' /\ meminj_valid j23' L2 m2' L3 m3' /\*)
                              Mem.extends m1' m2' /\ mem_forward m2 m2' /\ Mem.inject j' m2' m3' /\
@@ -260,14 +285,16 @@ Proof.
 
   destruct (eff_after_external12 _ _ _ _ HasTy1 HasTy1 EXT12' (Val.lessdef_refl _) FwdSrc Fwd2 RDO1 RDO2 Unch2a)
     as [cd12 [st1' [st2'' [AftExt1 [AftExt2 MC12']]]]].
-  assert (InjValid23': meminj_valid j' L1 m2' L3 m3').
-  { destruct MV as [MVa [MVb MVc]].
+  assert (InjValid23': meminj_valid j' (M2,L1) (M3,L3) m2' m3').
+  { destruct MV as [MVa [MVb [MVc [MVd MVe]]]].
     split; intros.
       apply (Mem.valid_block_extends _ _ _ EXT12'); apply (MVa _ H).
     split; intros.
       apply MVb; trivial.
-    destruct (MVc _ _ _ J).
-      apply (Mem.valid_block_extends _ _ _ EXT12') in H. split; trivial. } 
+    split; intros. destruct (MVc _ _ _ J).
+      apply (Mem.valid_block_extends _ _ _ EXT12') in H. split; trivial.
+    split; trivial.
+    intros. destruct (MV12c _ _ H). split; trivial. apply Fwd2; trivial. } 
 
   assert (UnchTgt_OOR: Mem.unchanged_on (BuiltinEffects.o_o_reach j L3 m2) m3 m3').
   { split; intros.
@@ -285,7 +312,7 @@ Proof.
   exists ((cd12, Some st2'), cd23), st1', st3'.
   split. assumption.
   split. assumption.
-  exists st2', m2'. split; trivial. split; trivial. }
+  exists st2', m2', M2. split; trivial. split; trivial. }
 Admitted. (*remaining admits are about readonly or at global blocks*)  
 
 End EI_sim_trans. 
